theories/simplang/derived.v
@@ -1,0 +1,73 @@
+(** This file extends the HeapLang program logic with some derived laws (not
+using the lifting lemmas) about arrays and prophecies.
+
+For utility functions on arrays (e.g., freeing/copying an array), see
+[heap_lang.lib.array].  *)
+
+From stdpp Require Import fin_maps.
+From iris.bi Require Import lib.fractional.
+From iris.proofmode Require Import tactics.
+From simuliris.simulation Require Export slsls.
+From simuliris.simplang Require Export primitive_laws.
+From simuliris.simplang Require Import tactics notation.
+From iris.prelude Require Import options.
+
+(** The [array] connective is a version of [mapsto] that works
+with lists of values. *)
+(* again parameterized over the ghost names *)
+Definition array `{!sheapG Σ} {γh γm} {hG : gen_heapPreNameG loc (option val) Σ γh γm} (l : loc) (dq : dfrac) (vs : list val) : iProp Σ :=
+  ([∗ list] i ↦ v ∈ vs, mapsto (hG:=hG) (l +ₗ i)  dq (Some v%V))%I.
+
+(** FIXME: Refactor these notations using custom entries once Coq bug #13654
+has been fixed. *)
+Notation "l ↦t∗{ dq } vs" := (array (hG:=gen_heap_inG_target) l dq vs)
+  (at level 20, format "l  ↦t∗{ dq }  vs") : bi_scope.
+Notation "l ↦t∗□ vs" := (array (hG:=gen_heap_inG_target) l DfracDiscarded vs)
+  (at level 20, format "l  ↦t∗□  vs") : bi_scope.
+Notation "l ↦t∗{# q } vs" := (array (hG:=gen_heap_inG_target) l (DfracOwn q) vs)
+  (at level 20, format "l  ↦t∗{# q }  vs") : bi_scope.
+Notation "l ↦t∗ vs" := (array (hG:=gen_heap_inG_target) l (DfracOwn 1) vs)
+  (at level 20, format "l  ↦t∗  vs") : bi_scope.
+
+Notation "l ↦s∗{ dq } vs" := (array (hG:=gen_heap_inG_source) l dq vs)
+  (at level 20, format "l  ↦s∗{ dq }  vs") : bi_scope.
+Notation "l ↦s∗□ vs" := (array (hG:=gen_heap_inG_source) l DfracDiscarded vs)
+  (at level 20, format "l  ↦s∗□  vs") : bi_scope.
+Notation "l ↦s∗{# q } vs" := (array (hG:=gen_heap_inG_source) l (DfracOwn q) vs)
+  (at level 20, format "l  ↦s∗{# q }  vs") : bi_scope.
+Notation "l ↦s∗ vs" := (array (hG:=gen_heap_inG_source) l (DfracOwn 1) vs)
+  (at level 20, format "l  ↦s∗  vs") : bi_scope.
+
+
+(** * Rules for allocation *)
+Lemma mapsto_seq_array `{sheapG Σ} {γh γm} {hG : gen_heapPreNameG loc (option val) Σ γh γm} l dq v n :
+  ([∗ list] i ∈ seq 0 n, mapsto (hG:=hG) (l +ₗ (i : nat)) dq (Some v)) -∗
+  array (hG:=hG) l dq (replicate n v).
+Proof.
+  rewrite /array. iInduction n as [|n'] "IH" forall (l); simpl.
+  { done. }
+  iIntros "[$ Hl]". rewrite -fmap_S_seq big_sepL_fmap.
+  setoid_rewrite Nat2Z.inj_succ. setoid_rewrite <-Z.add_1_l.
+  setoid_rewrite <-loc_add_assoc. iApply "IH". done.
+Qed.
+
+Lemma target_red_allocN `{sheapG Σ} v n Ψ :
+  (0 < n)%Z →
+  (∀ l, l ↦t∗ replicate (Z.to_nat n) v -∗ target_red (of_val #l) Ψ) -∗
+  target_red (AllocN (Val $ LitV $ LitInt $ n) (Val v)) Ψ.
+Proof.
+  iIntros (Hzs) "Ht". iApply target_red_allocN_seq; [done..|].
+  iIntros (l) "Hlm". iApply "Ht". by iApply mapsto_seq_array.
+Qed.
+
+Lemma source_red_allocN `{sheapG Σ} v n Ψ :
+  (0 < n)%Z →
+  (∀ l, l ↦s∗ replicate (Z.to_nat n) v -∗ source_red (of_val #l) Ψ) -∗
+  source_red (AllocN (Val $ LitV $ LitInt $ n) (Val v)) Ψ.
+Proof.
+  iIntros (Hzs) "Ht". iApply source_red_allocN_seq; [done..|].
+  iIntros (l) "Hlm". iApply "Ht". by iApply mapsto_seq_array.
+Qed.
+
+
+(* TODO: more laws *)
