theories/simplang/proofmode.v
@@ -2,7 +2,11 @@ From iris.proofmode Require Import coq_tactics reduction.
 From iris.proofmode Require Export tactics.
 From simuliris.simulation Require Import slsls lifting language.
 From simuliris.simplang Require Import tactics class_instances.
-From simuliris.simplang Require Export notation primitive_laws.
+From simuliris.simplang Require Export notation primitive_laws derived.
+From iris.bi Require Import bi.
+Import bi.
+From iris.bi Require Import derived_laws.
+Import bi.
 From iris.prelude Require Import options.
 
 
@@ -17,31 +21,66 @@ Lemma tac_sim_expr_eval Δ Φ e_t e_t' e_s e_s' :
   envs_entails Δ (e_t' ⪯ e_s' {{ Φ }}) → envs_entails Δ (e_t ⪯ e_s {{ Φ }}).
 Proof. by intros -> ->. Qed.
 
-Lemma tac_sim_pure_target Δ n e_t e_t' e_s K_t Φ (ϕ : Prop):
+Lemma tac_target_red_expr_eval Δ Ψ e_t e_t' :
+  (∀ (e_t'':=e_t'), e_t = e_t'') →
+  envs_entails Δ (target_red e_t' Ψ : iProp Σ) →
+  envs_entails Δ (target_red e_t Ψ).
+Proof. by intros ->. Qed.
+
+Lemma tac_source_red_expr_eval Δ Ψ e_s e_s' :
+  (∀ (e_s'':=e_s'), e_s = e_s'') →
+  envs_entails Δ (source_red e_s' Ψ : iProp Σ) →
+  envs_entails Δ (source_red e_s Ψ).
+Proof. by intros ->. Qed.
+
+Lemma tac_target_red_pure Δ n e_t e_t' K_t Ψ (ϕ : Prop):
   PureExec ϕ n (e_t) (e_t') →
   ϕ →
-  envs_entails Δ ((fill K_t e_t') ⪯ e_s {{Φ}}) →
-  envs_entails Δ ((fill K_t e_t) ⪯ e_s {{Φ}}).
+  envs_entails Δ (target_red (fill K_t e_t') Ψ : iProp Σ) →
+  envs_entails Δ (target_red (fill K_t e_t) Ψ).
 Proof.
   intros ? ?. rewrite envs_entails_eq.
   (* We want [pure_exec_fill] to be available to TC search locally. *)
   pose proof @pure_exec_ctx.
-  rewrite sim_pure_step_target //.
+  rewrite target_red_lift_pure //.
 Qed.
 
-Lemma tac_sim_pure_source Δ n e_s e_s' e_t K_s Φ (ϕ : Prop):
+Lemma tac_source_red_pure Δ n e_s e_s' K_s Ψ (ϕ : Prop):
   PureExec ϕ n e_s e_s' →
   ϕ →
-  envs_entails Δ (e_t ⪯ (fill K_s e_s') {{Φ}}) →
-  envs_entails Δ (e_t ⪯ (fill K_s e_s) {{Φ}}).
+  envs_entails Δ (source_red (fill K_s e_s') Ψ : iProp Σ) →
+  envs_entails Δ (source_red (fill K_s e_s) Ψ).
 Proof.
   intros ? ?. rewrite envs_entails_eq.
   (* We want [pure_exec_fill] to be available to TC search locally. *)
   pose proof @pure_exec_ctx.
-  rewrite sim_pure_step_source //.
+  rewrite source_red_lift_pure //.
 Qed.
 
-Lemma tac_sim_value v_t v_s Φ Δ:
+Lemma tac_target_red_base e_t Ψ Δ :
+  envs_entails Δ (|==> Ψ e_t : iProp Σ) → envs_entails Δ (target_red e_t Ψ).
+Proof.
+  rewrite envs_entails_eq => ->. iIntros "H". by iApply target_red_base.
+Qed.
+Lemma tac_target_red_base_no_bupd e_t Ψ Δ :
+  envs_entails Δ (Ψ e_t : iProp Σ) → envs_entails Δ (target_red e_t Ψ).
+Proof.
+  rewrite envs_entails_eq => ->. iIntros "H". by iApply target_red_base.
+Qed.
+
+Lemma tac_source_red_base e_s Ψ Δ :
+  envs_entails Δ (∀ P_s σ_s, |==> Ψ P_s e_s σ_s : iProp Σ) → envs_entails Δ (source_red e_s Ψ).
+Proof.
+  rewrite envs_entails_eq => ->. iIntros "H". by iApply source_red_base.
+Qed.
+Lemma tac_source_red_base_no_bupd e_s Ψ Δ :
+  envs_entails Δ (∀ P_s σ_s, Ψ P_s e_s σ_s : iProp Σ) → envs_entails Δ (source_red e_s Ψ).
+Proof.
+  rewrite envs_entails_eq => ->. iIntros "H". iApply source_red_base.
+  iIntros (??). iModIntro; eauto.
+Qed.
+
+Lemma tac_sim_value v_t v_s Φ Δ :
   envs_entails Δ (|==> Φ v_t v_s) → envs_entails Δ (Val v_t ⪯ Val v_s {{ Φ }}).
 Proof.
   rewrite envs_entails_eq => ->. iIntros "H". iApply sim_bupd. by iApply sim_value.
@@ -60,8 +99,255 @@ Proof.
   rewrite envs_entails_eq=> -> ->. intros H.
   iIntros "H". iApply (sim_bind Ω e_t e_s K_t K_s Φ). by iApply H.
 Qed.
+
+Lemma tac_target_red_allocN n v j K Ψ Δ :
+  (0 < n)%Z →
+  (∀ l,
+    match envs_app false (Esnoc Enil j (array (hG:=gen_heap_inG_target) l (DfracOwn 1) (replicate (Z.to_nat n) v))) Δ with
+    | Some Δ' =>
+       envs_entails Δ' (target_red (fill K (Val $ LitV $ LitLoc l)) Ψ)
+    | None => False
+    end) →
+  envs_entails Δ (target_red (fill K (AllocN (Val $ LitV $ LitInt n) (Val v))) Ψ).
+Proof.
+  rewrite envs_entails_eq=> ? HΔ. iIntros "He".
+  iApply target_red_bind. iApply target_red_allocN; first done.
+  iIntros (l) "Hl". specialize (HΔ l).
+  destruct (envs_app _ _ _) as [Δ'|] eqn:HΔ'; [ | contradiction ].
+  iApply target_red_base. iModIntro. iExists #l; iSplitR; first done.
+  iApply HΔ.
+  rewrite envs_app_sound //; simpl. iApply "He"; eauto.
+Qed.
+
+Lemma tac_source_red_allocN n v j K Ψ Δ :
+  (0 < n)%Z →
+  (∀ l,
+    match envs_app false (Esnoc Enil j (array (hG:=gen_heap_inG_source) l (DfracOwn 1) (replicate (Z.to_nat n) v))) Δ with
+    | Some Δ' =>
+       envs_entails Δ' (source_red (fill K (Val $ LitV $ LitLoc l)) Ψ)
+    | None => False
+    end) →
+  envs_entails Δ (source_red (fill K (AllocN (Val $ LitV $ LitInt n) (Val v))) Ψ).
+Proof.
+  rewrite envs_entails_eq=> ? HΔ. iIntros "He".
+  iApply source_red_bind. iApply source_red_allocN; first done.
+  iIntros (l) "Hl". specialize (HΔ l).
+  destruct (envs_app _ _ _) as [Δ'|] eqn:HΔ'; [ | contradiction ].
+  iApply source_red_base; iIntros (??). iModIntro. iExists #l; iSplitR; first done.
+  iApply HΔ. rewrite envs_app_sound //; simpl. iApply "He"; eauto.
+Qed.
+
+Lemma tac_target_red_alloc v j K Ψ Δ :
+  (∀ l,
+    match envs_app false (Esnoc Enil j (l ↦t v)) Δ with
+    | Some Δ' =>
+       envs_entails Δ' (target_red (fill K (Val $ LitV $ LitLoc l)) Ψ)
+    | None => False
+    end) →
+  envs_entails Δ (target_red (fill K (Alloc (Val v))) Ψ).
+Proof.
+  rewrite envs_entails_eq=> HΔ. iIntros "He".
+  iApply target_red_bind. iApply target_red_alloc.
+  iIntros (l) "Hl". specialize (HΔ l).
+  destruct (envs_app _ _ _) as [Δ'|] eqn:HΔ'; [ | contradiction ].
+  iApply target_red_base. iModIntro. iExists #l; iSplitR; first done.
+  iApply HΔ.
+  rewrite envs_app_sound //; simpl. iApply "He"; eauto.
+Qed.
+
+Lemma tac_source_red_alloc v j K Ψ Δ :
+  (∀ l,
+    match envs_app false (Esnoc Enil j (l ↦s v)) Δ with
+    | Some Δ' =>
+       envs_entails Δ' (source_red (fill K (Val $ LitV $ LitLoc l)) Ψ)
+    | None => False
+    end) →
+  envs_entails Δ (source_red (fill K (Alloc (Val v))) Ψ).
+Proof.
+  rewrite envs_entails_eq=> HΔ. iIntros "He".
+  iApply source_red_bind. iApply source_red_alloc.
+  iIntros (l) "Hl". specialize (HΔ l).
+  destruct (envs_app _ _ _) as [Δ'|] eqn:HΔ'; [ | contradiction ].
+  iApply source_red_base; iIntros (??). iModIntro. iExists #l; iSplitR; first done.
+  iApply HΔ.
+  rewrite envs_app_sound //; simpl. iApply "He"; eauto.
+Qed.
+
+Lemma tac_target_red_free l v i K Ψ Δ :
+  envs_lookup i Δ = Some (false, l ↦t v)%I →
+  (let Δ' := envs_delete false i false Δ in
+    envs_entails Δ' (target_red (fill K (Val $ LitV LitUnit)) Ψ)) →
+  envs_entails Δ (target_red (fill K (Free (LitV l))) Ψ).
+Proof.
+  rewrite envs_entails_eq=> Hlk Hfin.
+  rewrite -target_red_bind. eapply wand_apply; first exact: target_red_free.
+  rewrite envs_lookup_split //; simpl.
+  iIntros "H". iApply sep_mono_r.
+  { iIntros "H". iApply target_red_base. iModIntro. iExists (#()); iSplitR; first done. iApply "H". }
+  rewrite -Hfin.
+  rewrite (envs_lookup_sound' _ _ _ _ _ Hlk).
+  by rewrite wand_elim_r.
+Qed.
+
+Lemma tac_source_red_free l v i K Ψ Δ :
+  envs_lookup i Δ = Some (false, l ↦s v)%I →
+  (let Δ' := envs_delete false i false Δ in
+    envs_entails Δ' (source_red (fill K (Val $ LitV LitUnit)) Ψ)) →
+  envs_entails Δ (source_red (fill K (Free (LitV l))) Ψ).
+Proof.
+  rewrite envs_entails_eq=> Hlk Hfin.
+  rewrite -source_red_bind. eapply wand_apply; first exact: source_red_free.
+  rewrite envs_lookup_split //; simpl.
+  iIntros "H". iApply sep_mono_r.
+  { iIntros "H". iApply source_red_base; iIntros (??). iModIntro. iExists (#()); iSplitR; first done. iApply "H". }
+  rewrite -Hfin.
+  rewrite (envs_lookup_sound' _ _ _ _ _ Hlk).
+  by rewrite wand_elim_r.
+Qed.
+
+Lemma tac_target_red_load Δ i K b l q v Ψ :
+  envs_lookup i Δ = Some (b, l ↦t{q} v)%I →
+  envs_entails Δ (target_red (fill K (Val v)) Ψ) →
+  envs_entails Δ (target_red (fill K (Load (LitV l))) Ψ).
+Proof.
+  rewrite envs_entails_eq=> ? Hi.
+  rewrite -target_red_bind. eapply wand_apply; first exact: target_red_load.
+  rewrite envs_lookup_split //; simpl.
+  destruct b; simpl.
+  * iIntros "[#$ He]". iIntros "_". iApply target_red_base. iModIntro. iExists v; iSplit; first done.
+    iApply Hi. iApply "He". iFrame "#".
+  * apply sep_mono_r, wand_mono; first done. rewrite Hi. iIntros "Ht".
+    iApply target_red_base; eauto.
+Qed.
+
+Lemma tac_source_red_load Δ i K b l q v Ψ :
+  envs_lookup i Δ = Some (b, l ↦s{q} v)%I →
+  envs_entails Δ (source_red (fill K (Val v)) Ψ) →
+  envs_entails Δ (source_red (fill K (Load (LitV l))) Ψ).
+Proof.
+  rewrite envs_entails_eq=> ? Hi.
+  rewrite -source_red_bind. eapply wand_apply; first exact: source_red_load.
+  rewrite envs_lookup_split //; simpl.
+  destruct b; simpl.
+  * iIntros "[#$ He]". iIntros "_". iApply source_red_base; iIntros (??). iModIntro. iExists v; iSplit; first done.
+    iApply Hi. iApply "He". iFrame "#".
+  * apply sep_mono_r, wand_mono; first done. rewrite Hi. iIntros "Hs".
+    iApply source_red_base; eauto.
+Qed.
+
+Lemma tac_target_red_store Δ i K l v v' Ψ :
+  envs_lookup i Δ = Some (false, l ↦t v)%I →
+  match envs_simple_replace i false (Esnoc Enil i (l ↦t v')) Δ with
+  | Some Δ' => envs_entails Δ' (target_red (fill K (Val $ LitV LitUnit)) Ψ)
+  | None => False
+  end →
+  envs_entails Δ (target_red (fill K (Store (LitV l) (Val v'))) Ψ).
+Proof.
+  rewrite envs_entails_eq=> ? Hi.
+  destruct (envs_simple_replace _ _ _) as [Δ'|] eqn:HΔ'; [ | contradiction ].
+  rewrite -target_red_bind. eapply wand_apply; first by eapply target_red_store.
+  rewrite envs_simple_replace_sound //; simpl.
+  rewrite right_id. apply sep_mono_r, wand_mono; first done.
+  rewrite Hi. iIntros "Ht". iApply target_red_base; eauto.
+Qed.
+
+Lemma tac_source_red_store Δ i K l v v' Ψ :
+  envs_lookup i Δ = Some (false, l ↦s v)%I →
+  match envs_simple_replace i false (Esnoc Enil i (l ↦s v')) Δ with
+  | Some Δ' => envs_entails Δ' (source_red (fill K (Val $ LitV LitUnit)) Ψ)
+  | None => False
+  end →
+  envs_entails Δ (source_red (fill K (Store (LitV l) (Val v'))) Ψ).
+Proof.
+  rewrite envs_entails_eq=> ? Hi.
+  destruct (envs_simple_replace _ _ _) as [Δ'|] eqn:HΔ'; [ | contradiction ].
+  rewrite -source_red_bind. eapply wand_apply; first by eapply source_red_store.
+  rewrite envs_simple_replace_sound //; simpl.
+  rewrite right_id. apply sep_mono_r, wand_mono; first done.
+  rewrite Hi. iIntros "Hs". iApply source_red_base; eauto.
+Qed.
+
+Lemma tac_to_target Δ e_t e_s Φ :
+  envs_entails Δ (target_red e_t (λ e_t', e_t' ⪯ e_s {{ Φ }}))%I →
+  envs_entails Δ (e_t ⪯ e_s {{ Φ }}).
+Proof. rewrite envs_entails_eq=> Hi. by rewrite -target_red_sim. Qed.
+
+Lemma tac_to_source Δ e_t e_s Φ :
+  envs_entails Δ (source_red e_s (λ _ e_s' _, e_t ⪯ e_s' {{ Φ }}))%I →
+  envs_entails Δ (e_t ⪯ e_s {{ Φ }}).
+Proof. rewrite envs_entails_eq=> Hi. by rewrite -source_red_sim. Qed.
+
+
+Lemma tac_target_to_sim Δ e_t e_s Φ :
+  envs_entails Δ (e_t ⪯ e_s {{ Φ }}) →
+  envs_entails Δ (target_red e_t (λ e_t', e_t' ⪯ e_s {{ Φ }}))%I.
+Proof.
+  rewrite envs_entails_eq=> Hi. rewrite -target_red_base.
+  iIntros "He". iModIntro. by iApply Hi.
+Qed.
+
+Lemma tac_source_to_sim Δ e_t e_s Φ :
+  envs_entails Δ (e_t ⪯ e_s {{ Φ }}) →
+  envs_entails Δ (source_red e_s (λ _ e_s' _, e_t ⪯ e_s' {{ Φ }}))%I.
+Proof.
+  rewrite envs_entails_eq=> Hi. rewrite -source_red_base.
+  iIntros "He" (??). iModIntro. by iApply Hi.
+Qed.
+
 End sim.
 
+(** ** automation for source_red and target_red *)
+Ltac to_sim :=
+  iStartProof;
+  lazymatch goal with
+  | |- envs_entails _ (sim _ _ _ _) => idtac
+  | |- envs_entails _ (target_red ?e_t _) =>
+      notypeclasses refine (tac_target_to_sim _ _ e_t _ _ _)
+  | |- envs_entails _ (source_red ?e_s _) =>
+      notypeclasses refine (tac_source_to_sim _ _ _ e_s _ _)
+  | _ => fail "not a target_eval or source_eval of suitable shape"
+  end.
+
+Ltac to_target :=
+  iStartProof;
+  to_sim;
+  lazymatch goal with
+  | |- envs_entails _ (sim ?Ω ?e_t ?e_s ?Φ) =>
+      notypeclasses refine (tac_to_target  Ω _ e_t e_s Φ _)
+  | _ => fail "to_target: not a sim"
+  end.
+
+Ltac to_source :=
+  iStartProof;
+  to_sim;
+  lazymatch goal with
+  | |- envs_entails _ (sim ?Ω ?e_t ?e_s ?Φ) =>
+      notypeclasses refine (tac_to_source  Ω _ e_t e_s Φ _)
+  | _ => fail "to_source: not a sim"
+  end.
+
+(** ** simple automation for evaluation *)
+Ltac solve_vals_compare_safe :=
+  (* The first branch is for when we have [vals_compare_safe] in the context.
+     The other two branches are for when either one of the branches reduces to
+     [True] or we have it in the context. *)
+  fast_done || (left; fast_done) || (right; fast_done).
+
+(** Simplify the goal if it is [sim] of a value.
+  If the postcondition already allows a bupd, do not add a second one.
+  But otherwise, *do* add a bupd. This ensures that all the lemmas applied
+  here are bidirectional, so we never will make a goal unprovable. *)
+Ltac sim_value_head :=
+  lazymatch goal with
+  | |- envs_entails _ (sim _ (Val _) (Val _) (λ _ _, bupd _)) =>
+      eapply tac_sim_value_no_bupd
+  | |- envs_entails _ (sim _ (Val _) (Val _) (λ _ _, sim _ _ _ _)) =>
+      eapply tac_sim_value_no_bupd
+  | |- envs_entails _ (sim _ (Val _) (Val _) _) =>
+      eapply tac_sim_value
+  end.
+
+(* TODO: do we even need this? *)
 Tactic Notation "sim_expr_eval" tactic3(t) :=
   iStartProof;
   lazymatch goal with
@@ -72,31 +358,65 @@ Tactic Notation "sim_expr_eval" tactic3(t) :=
   end.
 Ltac sim_expr_simpl := sim_expr_eval simpl.
 
-Ltac solve_vals_compare_safe :=
-  (* The first branch is for when we have [vals_compare_safe] in the context.
-     The other two branches are for when either one of the branches reduces to
-     [True] or we have it in the context. *)
-  fast_done || (left; fast_done) || (right; fast_done).
-
-
-(** Simplify the goal if it is [sim] of a value.
-  If the postcondition already allows a bupd, do not add a second one.
-  But otherwise, *do* add a bupd. This ensures that all the lemmas applied
-  here are bidirectional, so we never will make a goal unprovable. *)
-Ltac sim_value_head :=
-  lazymatch goal with
-  | |- envs_entails _ (sim _ (Val _) (Val _) (λ _ _, bupd _)) =>
-      eapply tac_sim_value_no_bupd
-  | |- envs_entails _ (sim _ (Val _) (Val _) (λ _ _, sim _ _ _)) =>
-      eapply tac_sim_value_no_bupd
-  | |- envs_entails _ (sim _ (Val _) (Val _) _) =>
-      eapply tac_sim_value
-  end.
-
 Ltac sim_finish :=
+  (* TODO: can remove sim_expr_simpl if we do not use sim_finish anywhere explicitly *)
   sim_expr_simpl;      (* simplify occurences of subst/fill *)
   try sim_value_head;  (* in case we have reached a value, get rid of the WP *)
   pm_prettify.        (* prettify λs caused by wp_value *)
+
+
+(** target_red *)
+Tactic Notation "target_red_expr_eval" tactic3(t) :=
+  iStartProof;
+  lazymatch goal with
+  | |- envs_entails _ (target_red ?e_t ?Ψ) =>
+    notypeclasses refine (tac_target_red_expr_eval _ _ e_t _ _ _);
+      [let x := fresh in intros x; t; unfold x; notypeclasses refine eq_refl| ]
+  | _ => fail "target_red_expr_eval: not a 'target_red"
+  end.
+Ltac target_expr_simpl := target_red_expr_eval simpl.
+
+Ltac target_value_head :=
+  lazymatch goal with
+  | |- envs_entails _ (target_red (Val _) (λ _, bupd _)) =>
+      eapply tac_target_red_base_no_bupd
+  | |- envs_entails _ (target_red (Val _) (λ _, sim _ _ _ _)) =>
+      eapply tac_target_red_base_no_bupd
+  | |- envs_entails _ (target_red (Val _) _) =>
+      eapply tac_target_red_base
+  end.
+
+Ltac target_finish :=
+  target_expr_simpl;      (* simplify occurences of subst/fill *)
+  first [target_value_head; sim_finish | pm_prettify].
+
+(** source_red *)
+Tactic Notation "source_red_expr_eval" tactic3(t) :=
+  iStartProof;
+  lazymatch goal with
+  | |- envs_entails _ (source_red ?e_s ?Ψ) =>
+    notypeclasses refine (tac_source_red_expr_eval _ _ e_s _ _ _);
+      [let x := fresh in intros x; t; unfold x; notypeclasses refine eq_refl| ]
+  | _ => fail "source_red_expr_eval: not a 'target_red"
+  end.
+Ltac source_expr_simpl := source_red_expr_eval simpl.
+
+(* TODO: make more robust by using variant of source_red that takes predicates expr → iProp (instead of iIntros) *)
+Ltac source_value_head :=
+  lazymatch goal with
+  | |- envs_entails _ (source_red (Val _) (λ _ _ _, bupd _)) =>
+      eapply tac_source_red_base_no_bupd; try iIntros (_ _)
+  | |- envs_entails _ (source_red (Val _) (λ _ _ _, sim _ _ _ _)) =>
+      eapply tac_source_red_base_no_bupd; try iIntros (_ _)
+  | |- envs_entails _ (source_red (Val _) _) =>
+      eapply tac_source_red_base; try iIntros (_ _)
+  end.
+
+Ltac source_finish :=
+  source_expr_simpl;      (* simplify occurences of subst/fill *)
+  first [source_value_head; sim_finish | pm_prettify].
+
+(** ** Pure reduction *)
 
 (** The argument [efoc] can be used to specify the construct that should be
 reduced. For example, you can write [wp_pure (EIf _ _ _)], which will search
@@ -105,55 +425,57 @@ for an [EIf _ _ _] in the expression, and reduce it.
 The use of [open_constr] in this tactic is essential. It will convert all holes
 (i.e. [_]s) into evars, that later get unified when an occurences is found
 (see [unify e' efoc] in the code below). *)
-Tactic Notation "sim_pure_target" open_constr(efoc) :=
+Tactic Notation "target_red_pure" open_constr(efoc) :=
   iStartProof;
+  to_target;
   lazymatch goal with
-  | |- envs_entails _ (sim ?Ω ?e_t ?e_s ?Q) =>
+  | |- envs_entails _ (target_red ?e_t _) =>
     let e_t := eval simpl in e_t in
     reshape_expr e_t ltac:(fun K_t e_t' =>
       unify e_t' efoc;
-      eapply (tac_sim_pure_target Ω _ _ e_t' _ _ K_t _ _);
+      eapply (tac_target_red_pure _ _ e_t' _ K_t _ _);
       [ iSolveTC                       (* PureExec *)
       | try solve_vals_compare_safe    (* The pure condition for PureExec --
          handles trivial goals, including [vals_compare_safe] *)
-      | sim_finish                      (* new goal *)
+      | target_finish                      (* new goal *)
       ])
-    || fail "sim_pure_target: cannot find" efoc "in" e_t "or" efoc "is not a redex"
-  | _ => fail "sim_pure_target: not a 'sim'"
+    || fail "target_red_pure: cannot find" efoc "in" e_t "or" efoc "is not a redex"
+  | _ => fail "target_red_pure: not a 'target_red"
   end.
 
-Tactic Notation "sim_pure_source" open_constr(efoc) :=
+Tactic Notation "source_red_pure" open_constr(efoc) :=
   iStartProof;
+  to_source;
   lazymatch goal with
-  | |- envs_entails _ (sim ?Ω ?e_t ?e_s ?Q) =>
+  | |- envs_entails _ (source_red ?e_s _) =>
     let e_s := eval simpl in e_s in
     reshape_expr e_s ltac:(fun K_s e_s' =>
       unify e_s' efoc;
-      eapply (tac_sim_pure_source Ω _ _ e_s' _ _ K_s _ _);
+      eapply (tac_source_red_pure _ _ e_s' _ K_s _ _);
       [ iSolveTC                       (* PureExec *)
       | try solve_vals_compare_safe    (* The pure condition for PureExec --
          handles trivial goals, including [vals_compare_safe] *)
-      | sim_finish                      (* new goal *)
+      | source_finish                      (* new goal *)
       ])
-    || fail "sim_pure_source: cannot find" efoc "in" e_s "or" efoc "is not a redex"
-  | _ => fail "sim_pure_source: not a 'sim'"
+    || fail "source_red_pure: cannot find" efoc "in" e_s "or" efoc "is not a redex"
+  | _ => fail "source_red_pure: not a 'sim'"
   end.
 
-Ltac sim_pures_target :=
+Ltac target_red_pures :=
   iStartProof;
   first [ (* The `;[]` makes sure that no side-condition magically spawns. *)
-          progress repeat (sim_pure_target _; [])
-        | sim_finish (* In case sim_pure_target never ran, make sure we do the usual cleanup. *)
+          progress repeat (target_red_pure _; [])
+        | target_finish (* In case target_red_pure never ran, make sure we do the usual cleanup.*)
         ].
 
-Ltac sim_pures_source :=
+Ltac source_red_pures :=
   iStartProof;
   first [ (* The `;[]` makes sure that no side-condition magically spawns. *)
-          progress repeat (sim_pure_source _; [])
-        | sim_finish (* In case sim_pure_target never ran, make sure we do the usual cleanup. *)
+          progress repeat (source_red_pure _; [])
+        | source_finish (* In case source_red_pure never ran, make sure we do the usual cleanup.*)
         ].
 
-Ltac sim_pures := (try sim_pures_target); (try sim_pures_source).
+Ltac sim_pures := (try target_red_pures); (try source_red_pures); try to_sim.
 
 
 Ltac sim_bind_core K_t K_s :=
@@ -178,6 +500,22 @@ Tactic Notation "sim_bind" open_constr(efoc_t) open_constr(efoc_s) :=
   | _ => fail "sim_bind: not a 'sim"
   end.
 
+
+(** ** Heap automation *)
+(*Tactic Notation "target_store" :=*)
+  (*let solve_mapsto _ :=*)
+    (*let l := match goal with |- _ = Some (_, (?l ↦t{_} _)%I) => l end in*)
+    (*iAssumptionCore || fail "target_store: cannot find" l "↦t ?" in*)
+  (*sim_pures;*)
+  (*lazymatch goal with*)
+  (*| |- envs_entails _ (target_red ?Ψ ?e) =>*)
+    (*first*)
+      (*[reshape_expr e ltac:(fun K e' => eapply (tac_target_red_store _ _ K _ _ _ Ψ))*)
+      (*|fail 1 "wp_store: cannot find 'Store' in" e];*)
+    (*[solve_mapsto ()*)
+    (*|pm_reduce; first [sim_seq|wp_finish]]*)
+  (*| _ => fail "target_store: not a 'target_red"*)
+  (*end.*)
 
 
 (** ** Automation related to stuckness *)
